MutIndirection WIP

disk-betree/Marshalling.dfy
@@ -4,6 +4,7 @@ include "Message.dfy"
 include "ImplState.dfy"
 include "SSTable.dfy"
 include "../lib/Option.dfy"
+include "../lib/MutableMap.dfy"
 
 module Marshalling {
   import opened GenericMarshalling
@@ -31,12 +32,14 @@ module Marshalling {
   import MS = MapSpec
   import Keyspace = MS.Keyspace
 
+  import MM = MutableMap
+
   type Reference = BC.Reference
   type LBA = BC.LBA
   type Sector = ImplState.Sector
   type Message = M.Message
   type Key = BT.G.Key
-  type Node = ImplState.Node
+  type Node = BT.G.Node
 
   /////// Grammar
 
@@ -110,7 +113,7 @@ module Marshalling {
     forall i | 0 <= i < |buckets| :: CappedBucket(buckets[i])
   }
 
-  predicate method CappedNode(node: Node)
+  predicate method CappedNode(node: ImplState.Node)
   requires ImplState.WFNode(node)
   {
     && |node.buckets| <= CapNumBuckets() as int
@@ -183,14 +186,19 @@ module Marshalling {
 
   method {:fuel ValInGrammar,3} ValToLBAsAndSuccs(a: seq<V>) returns (s : Option<ImplState.MutIndirectionTable>)
   requires valToLBAsAndSuccs.requires(a)
-  ensures ImplState.IIndirectionTableOpt(s) == valToLBAsAndSuccs(a)
-  ensures fresh(s)
+  ensures (
+      && var table := ImplState.IIndirectionTableOpt(s);
+      && var inter := valToLBAsAndSuccs(a);
+      && if table.Some?
+         then (inter.Some? && table.value.lbas == inter.value.0 && table.value.graph == inter.value.1)
+         else inter.None?)
+  ensures s.Some? ==> fresh(s.value)
   {
     if |a| == 0 {
-      var newHashMap := new ResizingHashMap<(Option<LBA>, seq<Reference>)>;
+      var newHashMap := new MM.ResizingHashMap<(Option<LBA>, seq<Reference>)>(1024); // TODO(alattuada) magic numbers
       s := Some(newHashMap);
     } else {
-      var res := valToLBAsAndSuccs(DropLast(a));
+      var res := ValToLBAsAndSuccs(DropLast(a));
       match res {
         case Some(mutMap) => {
           var tuple := Last(a);
@@ -202,10 +210,11 @@ module Marshalling {
               s := None;
             }
             case Some(succs) => {
-              if ref in graph || lba == 0 || !LBAType.ValidAddr(lba) {
+              var graphRef := mutMap.Get(ref);
+              if graphRef.Some? || lba == 0 || !LBAType.ValidAddr(lba) {
                 s := None;
               } else {
-                mutMap.Insert(ref, (Some(lba), succs));
+                var _ := mutMap.Insert(ref, (Some(lba), succs));
                 s := Some(mutMap);
               }
             }
@@ -235,18 +244,20 @@ module Marshalling {
     }
   }
 
-  method GraphClosed(table: MutIndirectionTable) returns (result: bool)
-    requires BC.GraphClosed.requires(IIndirectionTable(table))
-    requires BC.GraphClosed(IIndirectionTable(table)) == result
+  method GraphClosed(table: ImplState.MutIndirectionTable) returns (result: bool)
+    requires BC.GraphClosed.requires(ImplState.IIndirectionTable(table).graph)
+    ensures BC.GraphClosed(ImplState.IIndirectionTable(table).graph) == result
 
   method ValToIndirectionTable(v: V) returns (s : Option<ImplState.MutIndirectionTable>)
-  requires ValInGrammar(v, IndirectionTableGrammar())
-  ensures s.Some? ==> BC.WFCompleteIndirectionTable(s.value)
+  requires valToIndirectionTable.requires(v)
+  ensures ImplState.IIndirectionTableOpt(s) == valToIndirectionTable(v)
   {
-    var res := valToLBAsAndSuccs(v.a);
+    var res := ValToLBAsAndSuccs(v.a);
     match res {
       case Some(res) => {
-        if res.Get(BT.G.Root()).Some? && GraphClosed(res) {
+        var rootRef := res.Get(BT.G.Root());
+        var isGraphClosed := GraphClosed(res);
+        if rootRef.Some? && isGraphClosed {
           s := Some(res);
         } else {
           s := None;
@@ -287,12 +298,10 @@ module Marshalling {
     s := ar[..];
   }
 
-  function {:fuel ValInGrammar,2} valToBucket(v: V, pivotTable: seq<Key>, i: int) : (s : Option<SSTable.SSTable>)
+  function {:fuel ValInGrammar,2} valToBucket(v: V, pivotTable: seq<Key>, i: int) : (s : Option<map<Key, Message>>)
   requires ValInGrammar(v, BucketGrammar())
   requires Pivots.WFPivots(pivotTable)
   requires 0 <= i <= |pivotTable|
-  ensures s.Some? ==> SSTable.WFSSTableMap(s.value)
-  ensures s.Some? ==> BT.WFBucket(SSTable.I(s.value), pivotTable, i)
   {
     var starts := valToUint64Seq(v.t[0].a);
 
@@ -300,14 +309,23 @@ module Marshalling {
     var sst := SSTable.SSTable(starts, strings);
 
     if SSTable.WFSSTableMap(sst) && BT.WFBucket(SSTable.I(sst), pivotTable, i) then
-      Some(sst)
+      Some(SSTable.I(sst))
+    else
+      None
+  }
+
+  function ISSTableOpt(table : Option<SSTable.SSTable>): Option<map<Key, Message>> {
+    if table.Some? then
+      Some(SSTable.I(table.value))
     else
       None
   }
 
   method ValToBucket(v: V, pivotTable: seq<Key>, i: int) returns (s : Option<SSTable.SSTable>)
   requires valToBucket.requires(v, pivotTable, i)
-  ensures s == valToBucket(v, pivotTable, i)
+  ensures ISSTableOpt(s) == valToBucket(v, pivotTable, i)
+  ensures s.Some? ==> SSTable.WFSSTableMap(s.value)
+  ensures s.Some? ==> BT.WFBucket(SSTable.I(s.value), pivotTable, i)
   {
     var starts := ValToUint64Seq(v.t[0].a);
 
@@ -390,13 +408,11 @@ module Marshalling {
       }
   }
 
-  function valToBuckets(a: seq<V>, pivotTable: seq<Key>) : (s : Option<seq<SSTable.SSTable>>)
+  function valToBuckets(a: seq<V>, pivotTable: seq<Key>) : (s : Option<seq<map<Key, Message>>>)
   requires Pivots.WFPivots(pivotTable)
   requires forall i | 0 <= i < |a| :: ValInGrammar(a[i], BucketGrammar())
   requires |a| <= |pivotTable| + 1
   ensures s.Some? ==> |s.value| == |a|
-  ensures s.Some? ==> forall i | 0 <= i < |s.value| :: SSTable.WFSSTableMap(s.value[i])
-  ensures s.Some? ==> forall i | 0 <= i < |s.value| :: BT.WFBucket(SSTable.I(s.value[i]), pivotTable, i)
   {
     if |a| == 0 then
       Some([])
@@ -427,16 +443,26 @@ module Marshalling {
     }
   }
 
+  function ISeqSSTableOpt(s : Option<seq<SSTable.SSTable>>): Option<seq<map<Key, Message>>>
+  {
+    if s.Some? then
+      Some(Apply(SSTable.I, s.value))
+    else
+      None
+  }
+
   method ValToBuckets(a: seq<V>, pivotTable: seq<Key>) returns (s : Option<seq<SSTable.SSTable>>)
   requires valToBuckets.requires(a, pivotTable)
-  ensures s == valToBuckets(a, pivotTable)
+  ensures ISeqSSTableOpt(s) == valToBuckets(a, pivotTable)
+  ensures s.Some? ==> forall i | 0 <= i < |s.value| :: SSTable.WFSSTableMap(s.value[i])
+  ensures s.Some? ==> forall i | 0 <= i < |s.value| :: BT.WFBucket(SSTable.I(s.value[i]), pivotTable, i)
   {
     var ar := new SSTable.SSTable[|a|];
 
     var i := 0;
     while i < |a|
     invariant 0 <= i <= |a|
-    invariant Some(ar[..i]) == valToBuckets(a[..i], pivotTable)
+    invariant ISeqSSTableOpt(Some(ar[..i])) == valToBuckets(a[..i], pivotTable)
     {
       var b := ValToBucket(a[i], pivotTable, i);
       if (b.None?) {
@@ -461,8 +487,7 @@ module Marshalling {
 
   function {:fuel ValInGrammar,2} valToNode(v: V) : (s : Option<Node>)
   requires ValInGrammar(v, PivotNodeGrammar())
-  ensures s.Some? ==> ImplState.WFNode(s.value)
-  ensures s.Some? ==> BT.WFNode(ImplState.INode(s.value))
+  ensures s.Some? ==> BT.WFNode(s.value)
   {
     match valToPivots(v.t[0].a) {
       case None => None
@@ -474,7 +499,7 @@ module Marshalling {
               match valToBuckets(v.t[2].a, pivots) {
                 case None => None
                 case Some(buckets) => (
-                  var node := ImplState.Node(pivots, if |children| == 0 then None else Some(children), buckets);
+                  var node := BT.G.Node(pivots, if |children| == 0 then None else Some(children), buckets);
                   Some(node)
                 )
               }
@@ -487,9 +512,18 @@ module Marshalling {
     }
   }
 
-  method ValToNode(v: V) returns (s : Option<Node>)
+  function INodeOpt(s : Option<ImplState.Node>): Option<Node>
+  {
+    if s.Some? then
+      Some(ImplState.INode(s.value))
+    else
+      None
+  }
+
+  method ValToNode(v: V) returns (s : Option<ImplState.Node>)
   requires valToNode.requires(v)
-  ensures s == valToNode(v)
+  ensures INodeOpt(s) == valToNode(v)
+  ensures s.Some? ==> ImplState.WFNode(s.value)
   {
     var pivotsOpt := valToPivots(v.t[0].a);
     if (pivotsOpt.None?) {
@@ -517,29 +551,38 @@ module Marshalling {
     return Some(node);
   }
 
-  function valToSector(v: V) : (s : Option<Sector>)
+  function valToSector(v: V) : (s : Option<BC.Sector>)
   requires ValInGrammar(v, SectorGrammar())
-  ensures s.Some? ==> ImplState.WFSector(s.value)
   {
     if v.c == 0 then (
       match valToIndirectionTable(v.val) {
-        case Some(s) => Some(ImplState.SectorIndirectionTable(s))
+        case Some(s) => Some(BC.SectorIndirectionTable(s))
         case None => None
       }
     ) else (
       match valToNode(v.val) {
-        case Some(s) => Some(ImplState.SectorBlock(s))
+        case Some(s) => Some(BC.SectorBlock(s))
         case None => None
       }
     )
   }
 
-  method ValToSector(v: V) returns (s : Option<Sector>)
+  function ISectorOpt(s : Option<ImplState.Sector>): Option<BC.Sector>
+  {
+    if s.Some? then
+      Some(ImplState.ISector(s.value))
+    else
+      None
+  }
+
+  method ValToSector(v: V) returns (s : Option<ImplState.Sector>)
   requires valToSector.requires(v)
-  ensures s == valToSector(v)
+  ensures ISectorOpt(s) == valToSector(v)
+  ensures s.Some? ==> ImplState.WFSector(s.value)
   {
     if v.c == 0 {
-      match valToIndirectionTable(v.val) {
+      var mutMap := ValToIndirectionTable(v.val);
+      match mutMap {
         case Some(s) => return Some(ImplState.SectorIndirectionTable(s));
         case None => return None;
       }
@@ -660,7 +703,7 @@ module Marshalling {
   ensures ValInGrammar(v, BucketGrammar())
   ensures SizeOfV(v) <= 8 + CapBucketNumEntries() as int * 8 + 8 + CapBucketSize() as int
   ensures ValidVal(v)
-  ensures valToBucket(v, pivotTable, i) == Some(bucket)
+  ensures valToBucket(v, pivotTable, i) == ISSTableOpt(Some(bucket))
   {
     var vstarts := uint64ArrayToVal(bucket.starts);
     return VTuple([
@@ -680,7 +723,7 @@ module Marshalling {
   ensures SizeOfV(v) <= 8 + |buckets| * (8 + CapBucketNumEntries() as int * 8 + 8 + CapBucketSize() as int)
   ensures ValInGrammar(v, GArray(BucketGrammar()))
   ensures |v.a| == |buckets|
-  ensures valToBuckets(v.a, pivotTable) == Some(buckets)
+  ensures valToBuckets(v.a, pivotTable) == ISeqSSTableOpt(Some(buckets))
   {
     if |buckets| == 0 {
       return VArray([]);
@@ -752,7 +795,7 @@ module Marshalling {
     }
   }
 
-  method {:fuel SizeOfV,4} nodeToVal(node: Node) returns (v : V)
+  method {:fuel SizeOfV,4} nodeToVal(node: ImplState.Node) returns (v : V)
   requires ImplState.WFNode(node)
   requires BT.WFNode(ImplState.INode(node))
   requires CappedNode(node)
@@ -762,7 +805,7 @@ module Marshalling {
       8 + (CapNumBuckets() as int - 1) * (8 + CapKeySize() as int) +
       8 + CapNumBuckets() as int * 8
   ensures ValInGrammar(v, PivotNodeGrammar())
-  ensures valToNode(v) == Some(node)
+  ensures valToNode(v) == INodeOpt(Some(node))
   {
     forall i | 0 <= i < |node.buckets|
     ensures BT.WFBucket(SSTable.I(node.buckets[i]), node.pivotTable, i);
@@ -786,20 +829,21 @@ module Marshalling {
     assert SizeOfV(v) == SizeOfV(pivots) + SizeOfV(children) + SizeOfV(buckets);
   }
 
-  method sectorToVal(sector: Sector) returns (v : Option<V>)
+  method sectorToVal(sector: ImplState.Sector) returns (v : Option<V>)
   requires ImplState.WFSector(sector)
   requires sector.SectorBlock? ==> BT.WFNode(ImplState.INode(sector.block))
   requires sector.SectorBlock? ==> CappedNode(sector.block);
   ensures v.Some? ==> ValidVal(v.value)
   ensures v.Some? ==> ValInGrammar(v.value, SectorGrammar());
-  ensures v.Some? ==> valToSector(v.value) == Some(sector)
+  ensures v.Some? ==> valToSector(v.value) == ISectorOpt(Some(sector))
   ensures sector.SectorBlock? ==> v.Some?
   ensures sector.SectorBlock? ==> SizeOfV(v.value) <= BlockSize() as int
   {
     match sector {
-      case SectorIndirectionTable(IndirectionTable(lbas, succs)) => {
-        if |lbas| < 0x1_0000_0000_0000_0000 {
-          var w := lbasSuccsToVal(lbas, succs);
+      case SectorIndirectionTable(mutMap) => {
+        var table := ImplState.IIndirectionTable(mutMap);
+        if |table.lbas| < 0x1_0000_0000_0000_0000 {
+          var w := lbasSuccsToVal(table.lbas, table.graph);
           match w {
             case Some(v) => return Some(VCase(0, v));
             case None => return None;
@@ -817,9 +861,7 @@ module Marshalling {
 
   /////// Marshalling and de-marshalling
 
-  function {:opaque} parseSector(data: seq<byte>) : (s : Option<Sector>)
-  ensures s.Some? ==> ImplState.WFSector(s.value)
-  ensures s.Some? && s.value.SectorBlock? ==> BT.WFNode(ImplState.INode(s.value.block))
+  function {:opaque} parseSector(data: seq<byte>) : (s : Option<BC.Sector>)
   {
     if |data| < 0x1_0000_0000_0000_0000 then (
       match parse_Val(data, SectorGrammar()).0 {
@@ -833,7 +875,7 @@ module Marshalling {
 
   method ParseSector(data: array<byte>) returns (s : Option<Sector>)
   requires data.Length < 0x1_0000_0000_0000_0000;
-  ensures s == parseSector(data[..])
+  ensures ISectorOpt(s) == parseSector(data[..])
   ensures s.Some? ==> ImplState.WFSector(s.value)
   ensures s.Some? && s.value.SectorBlock? ==> BT.WFNode(ImplState.INode(s.value.block))
   {
@@ -866,7 +908,7 @@ module Marshalling {
   requires ImplState.WFSector(sector)
   requires sector.SectorBlock? ==> BT.WFNode(ImplState.INode(sector.block))
   requires sector.SectorBlock? ==> CappedNode(sector.block);
-  ensures data != null ==> parseSector(data[..]) == Some(sector)
+  ensures data != null ==> parseSector(data[..]) == ISectorOpt(Some(sector))
   ensures data != null ==> data.Length == BlockSize() as int
   ensures sector.SectorBlock? ==> data != null;
   {
